ambig condition completeness

theories/ambiguity.v
@@ -13,39 +13,47 @@ Definition ambiguous {Σ N : Type} (G : grammar Σ N) :=
 
 (* bounded ambiguity *)
 
-Inductive sketch (Σ N : Type) (H : N) (h : sentence Σ) : Type :=
-  | hole : sketch Σ N H h
-  | unary_sketch : N → sketch Σ N H h → sketch Σ N H h
-  | left_sketch : N → sketch Σ N H h → tree Σ N → sketch Σ N H h
-  | right_sketch : N → tree Σ N → sketch Σ N H h → sketch Σ N H h
+Inductive sketch (Σ N : Type) : Type :=
+  | hole : N → sentence Σ → sketch Σ N
+  | unary_sketch : N → sketch Σ N → sketch Σ N
+  | left_sketch : N → sketch Σ N → tree Σ N → sketch Σ N
+  | right_sketch : N → tree Σ N → sketch Σ N → sketch Σ N
   .
 
-Arguments hole {_} {_} {_} {_}.
-Arguments unary_sketch {_} {_} {_} {_}.
-Arguments left_sketch {_} {_} {_} {_}.
-Arguments right_sketch {_} {_} {_} {_}.
+Arguments hole {_} {_}.
+Arguments unary_sketch {_} {_}.
+Arguments left_sketch {_} {_}.
+Arguments right_sketch {_} {_}.
 
-Definition sketch_root {Σ N : Type} {H h} (s : sketch Σ N H h) : N :=
+Definition sketch_root {Σ N : Type} (s : sketch Σ N) : N :=
   match s with
-  | hole => H
+  | hole H _ => H
   | unary_sketch R _ => R
   | left_sketch R _ _ => R
   | right_sketch R _ _ => R
   end.
 
-Fixpoint sketch_sentence {Σ N : Type} {H h} (s : sketch Σ N H h) : sentence Σ :=
+Fixpoint sketch_sentence {Σ N : Type} (s : sketch Σ N) : sentence Σ :=
   match s with
-  | hole => h
+  | hole _ h => h
   | unary_sketch _ s' => sketch_sentence s'
   | left_sketch _ s' t' => sketch_sentence s' ++ sentence_of t'
   | right_sketch _ t' s' => sentence_of t' ++ sketch_sentence s'
   end.
 
+Fixpoint hole_sig {Σ N : Type} (s : sketch Σ N) : N * sentence Σ :=
+  match s with
+  | hole H h => (H, h)
+  | unary_sketch _ s' => hole_sig s'
+  | left_sketch _ s' _ => hole_sig s'
+  | right_sketch _ _ s' => hole_sig s'
+  end.
+
 Reserved Notation "s ▷ₛ A ={ G }=> w" (at level 40, format "s  '▷ₛ'  A  '={' G '}=>'  w").
 
-Inductive sketch_witness {Σ N : Type} (G : grammar Σ N) {H h} : sketch Σ N H h → N → sentence Σ → Prop :=
-  | sketch_valid_hole :
-    hole ▷ₛ H ={G}=> h
+Inductive sketch_witness {Σ N : Type} (G : grammar Σ N) : sketch Σ N → N → sentence Σ → Prop :=
+  | sketch_valid_hole H h :
+    hole H h ▷ₛ H ={G}=> h
   | sketch_valid_unary A B φ s w :
     G ⊢ A ↦ unary B φ →
     s ▷ₛ B ={G}=> w →
@@ -65,15 +73,15 @@ Inductive sketch_witness {Σ N : Type} (G : grammar Σ N) {H h} : sketch Σ N H 
     right_sketch A t s ▷ₛ A ={G}=> (w1 ++ w2)
   where "s ▷ₛ A ={ G }=> w" := (sketch_witness G s A w).
 
-Fixpoint instantiate {Σ N : Type} {H h} (s : sketch Σ N H h) (t : tree Σ N) :=
+Fixpoint instantiate {Σ N : Type} (s : sketch Σ N) (t : tree Σ N) :=
   match s with
-  | hole => t
+  | hole _ _ => t
   | unary_sketch R s' => unary_tree R (instantiate s' t)
   | left_sketch R s' t' => binary_tree R (instantiate s' t) t'
   | right_sketch R t' s' => binary_tree R t' (instantiate s' t)
   end.
 
-Lemma instantiate_inj {Σ N H h} (s : sketch Σ N H h) :
+Lemma instantiate_inj {Σ N} (s : sketch Σ N) :
   Inj eq eq (instantiate s).
 Proof.
   move => t1 t2.
@@ -81,36 +89,46 @@ Proof.
   all: naive_solver.
 Qed.
 
-Lemma instantiate_witness {Σ N : Type} G {H h} (s : sketch Σ N H h) t A w :
+Lemma instantiate_witness {Σ N : Type} G H h (s : sketch Σ N) t A w :
+  hole_sig s = (H, h) →
   t ▷ H ={G}=> h →
   s ▷ₛ A ={G}=> w →
   instantiate s t ▷ A ={G}=> w.
 Proof.
-  move => Ht.
+  move => Hsig Ht.
   move : A w.
   induction s => A w Hs /=.
   all: inversion Hs; subst; clear Hs => //.
+  all: inversion Hsig; subst => //.
   all: econstructor => //; by apply IHs.
 Qed.
 
-Fixpoint sketch_subst {Σ N : Type} {H h H' h'} (s : sketch Σ N H h) (t : sketch Σ N H' h') : sketch Σ N H' h' :=
+Fixpoint sketch_subst {Σ N : Type} (s : sketch Σ N) (t : sketch Σ N) : sketch Σ N :=
   match s with
-  | hole => t
+  | hole _ _ => t
   | unary_sketch R s' => unary_sketch R (sketch_subst s' t)
   | left_sketch R s' t' => left_sketch R (sketch_subst s' t) t'
   | right_sketch R t' s' => right_sketch R t' (sketch_subst s' t)
   end.
 
-Lemma subst_witness {Σ N : Type} G {H h H' h'} (s : sketch Σ N H h) (t : sketch Σ N H' h') A w :
+Lemma subst_witness {Σ N : Type} G (s : sketch Σ N) (t : sketch Σ N) H h A w :
+  hole_sig s = (H, h) →
   t ▷ₛ H ={G}=> h →
   s ▷ₛ A ={G}=> w →
   sketch_subst s t ▷ₛ A ={G}=> w.
 Proof.
-  move => Ht.
+  move => Hsig Ht.
   move : A w.
   induction s => A w Hs /=.
   all: inversion Hs; subst; clear Hs => //.
+  all: inversion Hsig; subst => //.
   all: econstructor => //; by apply IHs.
+Qed.
+
+Lemma subst_hole_sig {Σ N : Type} (s : sketch Σ N) (t : sketch Σ N) :
+  hole_sig (sketch_subst s t) = hole_sig t.
+Proof.
+  by induction s.
 Qed.
 
 Definition similar {Σ N : Type} (t1 t2 : tree Σ N) : Prop :=
@@ -121,7 +139,7 @@ Definition similar {Σ N : Type} (t1 t2 : tree Σ N) : Prop :=
   | unary_tree R1 t1, unary_tree R2 t2 =>
     R1 = R2 ∧ root t1 = root t2
   | binary_tree R1 tA1 tB1, binary_tree R2 tA2 tB2 =>
-    R1 = R2 ∧ root tA1 = root tA2 ∧ root tB1 = root tB2
+    R1 = R2 ∧ root tA1 = root tA2 ∧ root tB1 = root tB2 ∧ sentence_of tA1 = sentence_of tA2
   | _, _ => False
   end.
 
@@ -132,13 +150,189 @@ Proof.
   destruct t => //=.
 Qed.
 
-Lemma sentence_ambiguous_iff {Σ N : Type} (G : grammar Σ N) w :
-  sentence_ambiguous G w ↔ ∃ H h (s : sketch Σ N H h),
-    s ▷ₛ (start G) ={G}=> w ∧ ∃ t1 t2, ¬ (similar t1 t2) ∧
+(* diff two trees with same root and sentence *)
+Fixpoint diff {Σ N : Type} `{EqDecision N} `{EqDecision (token Σ)}
+  (t1 t2 : tree Σ N) : option (tree Σ N * tree Σ N) :=
+  match t1, t2 with
+  | ε_tree _, ε_tree _ => None
+  | token_tree _ _, token_tree _ _ =>
+    (* tokens must be eq, so no diff *)
+    None
+  | unary_tree _ t1', unary_tree _ t2' =>
+    (* sentences must be eq, so just compare root *)
+    if bool_decide (root t1' = root t2')
+    then diff t1' t2'
+    else Some (t1, t2)
+  | binary_tree _ tl1 tr1, binary_tree _ tl2 tr2 =>
+    if bool_decide (root tl1 = root tl2 ∧ root tr1 = root tr2 ∧ sentence_of tl1 = sentence_of tl2)
+    then
+      match diff tl1 tl2 with
+      | Some p => Some p
+      | None => diff tr1 tr2
+      end
+    else Some (t1, t2)
+  | _, _ => Some (t1, t2)
+  end.
+
+Lemma diff_None {Σ N : Type} `{EqDecision N} `{EqDecision (token Σ)} (t1 t2 : tree Σ N) :
+  root t1 = root t2 →
+  sentence_of t1 = sentence_of t2 →
+  t1 = t2 ↔ diff t1 t2 = None.
+Proof.
+  intros. split.
+  - intros <-.
+    induction t1 => //=.
+    + case_bool_decide => //. by apply IHt1.
+    + case_bool_decide => //=.
+      * rewrite IHt1_1 => //. rewrite IHt1_2 => //.
+      * exfalso. naive_solver.
+  - generalize dependent t2.
+    induction t1 => t2.
+    all: destruct t2 => Hr Hw Hdiff //=.
+    1,2: naive_solver.
+    + simpl in Hr; subst.
+      simpl in Hdiff. case_bool_decide => //.
+      erewrite IHt1; eauto.
+    + simpl in Hr; subst.
+      simpl in Hdiff. case_bool_decide => //.
+      case_match => //.
+      erewrite (IHt1_1 t2_1).
+      erewrite (IHt1_2 t2_2).
+      all: eauto; naive_solver.
+Qed.
+
+Lemma diff_Some_inv {Σ N : Type} `{EqDecision N} `{EqDecision (token Σ)} (t1 t2 t1' t2' : tree Σ N) :
+  root t1 = root t2 →
+  sentence_of t1 = sentence_of t2 →
+  diff t1 t2 = Some (t1', t2') →
+  root t1' = root t2' ∧ sentence_of t1' = sentence_of t2'.
+Proof.
+  generalize dependent t2.
+  induction t1 => t2.
+  all: destruct t2 => //= -> Hw Hdiff.
+  all: inversion Hdiff; subst; clear Hdiff.
+  all: try naive_solver.
+  - case_bool_decide.
+    * eapply IHt1; eauto.
+    * inversion H0; subst; clear H0. done.
+  - case_bool_decide; first case_match.
+    * naive_solver.
+    * destruct H as [? [? ?]]. eapply (IHt1_2 t2_2); eauto.
+      rewrite H2 in Hw. by eapply app_inv_head_iff.
+    * naive_solver.
+Qed.
+
+Lemma diff_result_not_similar {Σ N : Type} `{EqDecision N} `{EqDecision (token Σ)} (t1 t2 t1' t2' : tree Σ N) :
+  diff t1 t2 = Some (t1', t2') → ¬ (similar t1' t2').
+Proof.
+  generalize dependent t2.
+  induction t1 => t2.
+  all: destruct t2 => //= Hdiff.
+  all: inversion Hdiff; subst; clear Hdiff.
+  all: try naive_solver.
+  - case_bool_decide; naive_solver.
+  - case_bool_decide; first case_match; naive_solver.
+Qed.
+
+Inductive subtree {Σ N : Type} : tree Σ N → tree Σ N → Prop :=
+  | subtree_refl t : subtree t t
+  | subtree_unary R t t' : 
+    subtree t t' →
+    subtree t (unary_tree R t')
+  | subtree_left R t tl tr :
+    subtree t tl →
+    subtree t (binary_tree R tl tr)
+  | subtree_right R t tl tr :
+    subtree t tr →
+    subtree t (binary_tree R tl tr)
+  .
+
+Lemma subtree_witness {Σ N : Type} (G : grammar Σ N) t t' A w :
+  subtree t' t →
+  t ▷ A ={ G }=> w →
+  t' ▷ (root t') ={ G }=> (sentence_of t').
+Admitted.
+
+Lemma subtree_sketch_intro {Σ N : Type} (G : grammar Σ N) t t' :
+  t ▷ (root t) ={ G }=> (sentence_of t) →
+  subtree t' t →
+  ∃ s, hole_sig s = (root t', sentence_of t') ∧ s ▷ₛ (root t) ={ G }=> (sentence_of t).
+Proof.
+  intros Ht.
+  induction 1.
+  - exists (hole (root t) (sentence_of t)).
+    split; first done.
+    constructor.
+  - edestruct IHsubtree as [s [? ?]].
+    { eapply subtree_witness; eauto. constructor. constructor. }
+    exists (unary_sketch R s).
+    split; first done.
+    inversion Ht; subst; clear Ht => /=.
+    econstructor; eauto.
+    have <- : root t' = B by inversion H5. done.
+  - edestruct IHsubtree as [s [? ?]].
+    { eapply subtree_witness; eauto. constructor. constructor. }
+    exists (left_sketch R s tr).
+    split; first done.
+    inversion Ht; subst; clear Ht => /=.
+    econstructor; eauto.
+    have <- : root tl = B1 by inversion H8. done.
+    have -> : sentence_of tr = w2 by admit. done.
+    admit.
+  - edestruct IHsubtree as [s [? ?]].
+    { eapply subtree_witness; eauto. apply subtree_right. constructor. }
+    exists (right_sketch R tl s).
+    split; first done.
+    inversion Ht; subst; clear Ht => /=.
+    econstructor; eauto.
+    admit. admit. admit.
+Admitted.
+
+Lemma diff_result_subtree {Σ N : Type} `{EqDecision N} `{EqDecision (token Σ)} (t1 t2 t1' t2' : tree Σ N) :
+  diff t1 t2 = Some (t1', t2') → subtree t1' t1 ∧ subtree t2' t2.
+Proof.
+  generalize dependent t2.
+  induction t1 => t2.
+  all: destruct t2 => //= Hdiff.
+  all: inversion Hdiff; subst; clear Hdiff.
+  all: try by split; constructor.
+  - case_bool_decide.
+    * edestruct IHt1; eauto. split; by constructor.
+    * inversion H0; subst. split; by constructor.
+  - case_bool_decide; first case_match.
+    * edestruct (IHt1_1 t2_1); eauto; try congruence. split; by constructor.
+    * edestruct (IHt1_2 t2_2); eauto. split; by constructor.
+    * inversion H0; subst. split; by constructor.
+Qed.
+
+Lemma sentence_ambiguous_iff {Σ N : Type} `{EqDecision N} `{EqDecision (token Σ)}
+  (G : grammar Σ N) w :
+  sentence_ambiguous G w ↔ ∃ H h (s : sketch Σ N),
+    s ▷ₛ (start G) ={G}=> w ∧ hole_sig s = (H, h) ∧ ∃ t1 t2, ¬ (similar t1 t2) ∧
       t1 ▷ H ={G}=> h ∧ t2 ▷ H ={G}=> h.
 Proof.
-  split. admit.
-  - move => [H [h [s [Hs [t1 [t2 [Hne [Ht1 Ht2]]]]]]]].
+  split.
+  - move => [t1 [t2 [Ht1 [Ht2 ?]]]].
+    have ? : root t1 = start G by inversion Ht1.
+    have ? : root t2 = start G by inversion Ht2.
+    have ? : sentence_of t1 = w by admit.
+    have ? : sentence_of t2 = w by admit.
+    have [[t1' t2'] Hdiff] : is_Some (diff t1 t2).
+    { apply not_eq_None_Some. intros Hcontra. apply diff_None in Hcontra => //.
+      all: congruence. }
+    have [Hsub1 Hsub2] := (diff_result_subtree _ _ _ _ Hdiff).
+    have Ht1' : t1 ▷ root t1 ={ G }=> sentence_of t1 by congruence.
+    have Ht2' : t2 ▷ root t2 ={ G }=> sentence_of t2 by congruence.
+    destruct (subtree_sketch_intro G _ _ Ht1' Hsub1) as [s [? ?]].
+    exists (root t1'), (sentence_of t1'), s.
+    split; first congruence.
+    split; first done.
+    exists t1', t2'. split; first by eapply diff_result_not_similar.
+    split; first by eapply subtree_witness; eauto.
+    have [-> ->] : root t1' = root t2' ∧ sentence_of t1' = sentence_of t2'.
+    { eapply diff_Some_inv; last eauto. all: congruence. }
+    eapply subtree_witness; eauto.
+  - move => [H [h [s [Hs [Hsig [t1 [t2 [Hne [Ht1 Ht2]]]]]]]]].
     eapply instantiate_witness in Ht1; eauto.
     eapply instantiate_witness in Ht2; eauto.
     exists (instantiate s t1), (instantiate s t2). repeat split => //.
@@ -172,22 +366,26 @@ Inductive reachable {Σ N : Type} (G : grammar Σ N) : N → sentence Σ → Pro
 
 Lemma reachable_sketch_intro {Σ N : Type} (G : grammar Σ N) H h :
   reachable G H h →
-  ∃ (s : sketch Σ N H h) w, s ▷ₛ (start G) ={G}=> w.
+  ∃ (s : sketch Σ N) w, hole_sig s = (H, h) ∧ s ▷ₛ (start G) ={G}=> w.
 Proof.
   induction 1; subst.
-  - exists hole, w. constructor.
-  - destruct IHreachable as [s' [w' ?]].
-    exists (sketch_subst s' (unary_sketch A hole)), w' => /=.
-    apply subst_witness => //.
+  - exists (hole (start G) w), w.
+    split; first done. constructor.
+  - destruct IHreachable as [s' [w' [? ?]]].
+    exists (sketch_subst s' (unary_sketch A (hole B w))), w' => /=.
+    split; first by rewrite subst_hole_sig.
+    eapply subst_witness => //.
     econstructor => //. constructor.
-  - destruct IHreachable as [sA [wA ?]].
+  - destruct IHreachable as [sA [wA [? ?]]].
     destruct H1 as [tB' ?].
-    exists (sketch_subst sA (left_sketch A hole tB')), wA => /=.
-    apply subst_witness => //.
+    exists (sketch_subst sA (left_sketch A (hole B w) tB')), wA => /=.
+    split; first by rewrite subst_hole_sig.
+    eapply subst_witness => //.
     econstructor => //. constructor.
-  - destruct IHreachable as [sA [wA ?]].
+  - destruct IHreachable as [sA [wA [? ?]]].
     destruct H1 as [tB' ?].
-    exists (sketch_subst sA (right_sketch A tB' hole)), wA => /=.
-    apply subst_witness => //.
+    exists (sketch_subst sA (right_sketch A tB' (hole B w))), wA => /=.
+    split; first by rewrite subst_hole_sig.
+    eapply subst_witness => //.
     econstructor => //. constructor.
 Qed.
